theories/Auth_max_nat.v
@@ -1,0 +1,91 @@
+From iris Require Export  algebra.auth algebra.numbers.
+From iris Require Import  algebra.excl base_logic.lib.own proofmode.tactics.
+
+
+
+Notation "'●max_nat' n" := (auth_auth (A:=max_natUR) 1%Qp n%nat) (at level 20).
+Notation "'◯max_nat' n" := (auth_frag (A:=max_natUR) n%nat) (at level 20).
+
+Local Coercion max_nat_car : max_nat >-> nat.
+
+Section Auth_max_nat.
+
+  Context `{inG Σ (authR max_natUR)}.
+
+  Lemma auth_max_nat_alloc (n : max_nat) :
+    ⊢ |==> ∃ γ, own γ (●max_nat n) ∗ own γ (◯max_nat n).
+  Proof.
+    iMod (own_alloc (●max_nat n ⋅ ◯max_nat n)) as (γ) "[? ?]".
+    - by apply auth_both_valid_2.
+    - by auto with iFrame.
+  Qed.
+  Global Arguments auth_max_nat_alloc _%nat.
+
+  Lemma own_auth_max_nat_le (γ : gname) (m n : max_nat) :
+    own γ (●max_nat m) -∗
+    own γ (◯max_nat n) -∗
+    ⌜(n ≤ m)%nat⌝.
+  Proof.
+    iIntros "H● H◯".
+    iDestruct (own_valid_2 with "H● H◯") as % [[k ->] _] % auth_both_valid.
+    iPureIntro. apply Max.le_max_l.
+  Qed.
+
+  Lemma own_auth_max_nat_weaken (γ : gname) (n₁ n₂ : max_nat) :
+    (n₂ ≤ n₁)%nat →
+    own γ (◯max_nat n₁) -∗
+    own γ (◯max_nat n₂).
+  Proof.
+    iIntros (I) "H".
+    rewrite (_ : n₁ = n₁ ⋅ n₂)%nat.
+    - iDestruct "H" as "[_$]".
+    - destruct n₁, n₂. rewrite max_nat_op_max. f_equal. simpl in I. lia.
+  Qed.
+  Global Arguments own_auth_max_nat_weaken _ (_ _ _)%nat_scope.
+
+  Lemma own_auth_max_nat_null (γ : gname) (m : max_nat) :
+    own γ (●max_nat m) -∗
+    own γ (●max_nat m) ∗ own γ (◯max_nat (MaxNat 0)).
+  Proof.
+    by rewrite - own_op.
+  Qed.
+  Global Arguments own_auth_max_nat_null _ _%nat_scope.
+
+  Lemma auth_max_nat_update_read_auth (γ : gname) (m : max_nat) :
+    own γ (●max_nat m) -∗
+    |==> own γ (●max_nat m) ∗ own γ (◯max_nat m).
+  Proof.
+    iIntros "H●".
+    iDestruct (own_auth_max_nat_null with "H●") as "[H● H◯]".
+    (iMod (own_update_2 with "H● H◯") as "[$ $]" ; last done).
+    apply auth_update, max_nat_local_update. lia.
+  Qed.
+  Global Arguments auth_max_nat_update_read_auth _ _%nat_scope.
+
+  Lemma auth_max_nat_update_incr (γ : gname) (m k : max_nat) :
+    own γ (●max_nat m) -∗
+    |==> own γ (●max_nat (MaxNat (m + k))).
+  Proof.
+    iIntros "H●". iDestruct (own_auth_max_nat_null with "H●") as "[H● H◯]".
+    iMod (own_update_2 with "H● H◯") as "[$ _]" ; last done.
+    apply auth_update, max_nat_local_update. destruct m. simpl. lia.
+  Qed.
+  Global Arguments auth_max_nat_update_incr _ (_ _)%nat_scope.
+
+  Lemma auth_max_nat_update_incr' (γ : gname) (m n k : max_nat) :
+    own γ (●max_nat m) -∗
+    own γ (◯max_nat n) -∗
+    |==> own γ (●max_nat (MaxNat (m + k))) ∗ own γ (◯max_nat (MaxNat (n + k))).
+  Proof.
+    iIntros "H● H◯".
+    iDestruct (own_auth_max_nat_le with "H● H◯") as %I. iClear "H◯".
+    iDestruct (auth_max_nat_update_incr _ _ k with "H●") as ">H●".
+    iDestruct (auth_max_nat_update_read_auth with "H●") as ">[$ H◯]".
+    iModIntro.
+    rewrite (_ : MaxNat (m + k) = MaxNat (n + k) ⋅ MaxNat (m + k))%nat.
+    - iDestruct "H◯" as "[$ _]".
+    - rewrite max_nat_op_max. f_equal. lia.
+  Qed.
+  Global Arguments auth_max_nat_update_incr' _ (_ _ _)%nat_scope.
+
+End Auth_max_nat.
