theories/Auth_nat.v
@@ -1,5 +1,5 @@
-From iris Require Export  algebra.auth.
-From iris Require Import  base_logic.lib.own  proofmode.tactics.
+From iris Require Export  algebra.auth algebra.numbers.
+From iris Require Import  base_logic.lib.own proofmode.tactics.
 
 
 
